vsSahlq/Coq code/List_machinery_impl.v
@@ -58,13 +58,13 @@ Fixpoint nlist_list_pred (n : nat) (ln : nlist_pred n) : list predicate :=
 
 (* --------------------------------------------------------------------------- *)
 
-(* Similar to altered_Ip but with list. *)
-Fixpoint altered_Ip_list {D:Set} (Ip: predicate -> D -> Prop) (l_pa : list (D -> Prop)) 
+(* Similar to alt_Ip but with list. *)
+Fixpoint alt_Ip_list {D:Set} (Ip: predicate -> D -> Prop) (l_pa : list (D -> Prop)) 
                       (l_pred : list (predicate)) : predicate -> D -> Prop:=
   match l_pa, l_pred with
     nil, _ => Ip
   | _, nil => Ip
-  | cons pa l_pa', cons P l_pred' =>  altered_Ip (altered_Ip_list Ip l_pa' l_pred') pa P
+  | cons pa l_pa', cons P l_pred' =>  alt_Ip (alt_Ip_list Ip l_pa' l_pred') pa P
   end.
 
 
@@ -254,10 +254,10 @@ Qed.
 
 (* ---------------------------------------------------------------------------- *)
 
-Lemma altered_Ip_eq : forall (W : Set) (Ip : predicate -> W -> Prop) (pa1 pa2 : W -> Prop)
+Lemma alt_Ip_eq : forall (W : Set) (Ip : predicate -> W -> Prop) (pa1 pa2 : W -> Prop)
                                  (P : predicate),
-     altered_Ip (altered_Ip Ip pa2 P) pa1 P 
-                    = altered_Ip Ip pa1 P.
+     alt_Ip (alt_Ip Ip pa2 P) pa1 P 
+                    = alt_Ip Ip pa1 P.
 Proof.
   intros.
   apply functional_extensionality.
@@ -275,10 +275,10 @@ Proof.
     reflexivity.
 Qed.
 
-Lemma altered_Ip_switch : forall (W : Set) (Ip : predicate -> W -> Prop) (pa1 pa2 : W -> Prop)
+Lemma alt_Ip_switch : forall (W : Set) (Ip : predicate -> W -> Prop) (pa1 pa2 : W -> Prop)
                                  (n m : nat),
-     ~(n = m) -> (altered_Ip (altered_Ip Ip pa2 (Pred m)) pa1 (Pred n) 
-                    = altered_Ip (altered_Ip Ip pa1 (Pred n)) pa2 (Pred m) ).
+     ~(n = m) -> (alt_Ip (alt_Ip Ip pa2 (Pred m)) pa1 (Pred n) 
+                    = alt_Ip (alt_Ip Ip pa1 (Pred n)) pa2 (Pred m) ).
 Proof.
   intros.
   apply functional_extensionality.
@@ -309,18 +309,18 @@ Qed.
 
 (* ------------------------------------------------------------------ *)
 
-Lemma altered_Ip_list_cons : forall (D:Set) (Ip: predicate -> D -> Prop) (l_pa : list (D -> Prop)) 
+Lemma alt_Ip_list_cons : forall (D:Set) (Ip: predicate -> D -> Prop) (l_pa : list (D -> Prop)) 
                       (l_pred : list (predicate)) (P : predicate) (pa : D -> Prop),
-            altered_Ip_list Ip (cons pa l_pa) (cons P l_pred) 
-               = altered_Ip (altered_Ip_list Ip l_pa l_pred) pa P.
+            alt_Ip_list Ip (cons pa l_pa) (cons P l_pred) 
+               = alt_Ip (alt_Ip_list Ip l_pa l_pred) pa P.
 Proof.
   intros.
   simpl.
   reflexivity.
 Qed.
 
-Lemma altered_Ip_list_nil : forall (D:Set) (Ip: predicate -> D -> Prop) (l_pa : list (D -> Prop)) ,
-  altered_Ip_list Ip l_pa nil = Ip.
+Lemma alt_Ip_list_nil : forall (D:Set) (Ip: predicate -> D -> Prop) (l_pa : list (D -> Prop)) ,
+  alt_Ip_list Ip l_pa nil = Ip.
 Proof.
   intros.  
   case l_pa.
@@ -331,11 +331,11 @@ Proof.
     reflexivity.
 Qed.
 
-Lemma altered_Ip_list_tail : forall (W : Set) (Ip : predicate -> W -> Prop) (P : predicate)
+Lemma alt_Ip_list_tail : forall (W : Set) (Ip : predicate -> W -> Prop) (P : predicate)
                             (l : list predicate) (pa_l : nlist_pa W (length l)) 
                             (pa: W -> Prop),
-         altered_Ip_list (altered_Ip Ip pa P) (nlist_list_pa W (length l) pa_l) l
-            = altered_Ip_list Ip (app (nlist_list_pa W (length l) pa_l) (cons pa nil) ) (app l (cons P nil)).
+         alt_Ip_list (alt_Ip Ip pa P) (nlist_list_pa W (length l) pa_l) l
+            = alt_Ip_list Ip (app (nlist_list_pa W (length l) pa_l) (cons pa nil) ) (app l (cons P nil)).
 Proof.
   intros.
   induction l.
@@ -357,11 +357,11 @@ Proof.
     reflexivity.
 Qed.
 
-Lemma altered_Ip_list_app : forall (W : Set) (Ip : predicate -> W -> Prop) (P : predicate)
+Lemma alt_Ip_list_app : forall (W : Set) (Ip : predicate -> W -> Prop) (P : predicate)
                             (l : list predicate) (pa_l : nlist_pa W (length l)) 
                             (pa : W -> Prop),
-       (altered_Ip_list Ip (app (nlist_list_pa W (length l) pa_l) (cons pa nil)) (l ++ P :: nil))
-     = (altered_Ip_list (altered_Ip_list Ip (nlist_list_pa W 1 (consn_pa W 0 pa (niln_pa W)))
+       (alt_Ip_list Ip (app (nlist_list_pa W (length l) pa_l) (cons pa nil)) (l ++ P :: nil))
+     = (alt_Ip_list (alt_Ip_list Ip (nlist_list_pa W 1 (consn_pa W 0 pa (niln_pa W)))
           (P :: nil)) (nlist_list_pa W (length l) pa_l) l).
 Proof.
   intros.
@@ -391,8 +391,8 @@ Qed.
 Lemma alt_alt_list_1 : forall (W : Set) (l : list predicate) (pa_l_hat : nlist_pa W (length l)) 
                             (pa_hat : W -> Prop) (P : predicate) (Ip : predicate -> W -> Prop) ,
       exists (pa : W -> Prop) (pa_l : nlist_pa W (length l)),
-          (altered_Ip (altered_Ip_list Ip (nlist_list_pa W (length l) pa_l_hat) l) pa_hat P) 
-        = (altered_Ip_list (altered_Ip Ip pa P) (nlist_list_pa W (length l) pa_l) l).
+          (alt_Ip (alt_Ip_list Ip (nlist_list_pa W (length l) pa_l_hat) l) pa_hat P) 
+        = (alt_Ip_list (alt_Ip Ip pa P) (nlist_list_pa W (length l) pa_l) l).
 Proof.
   intros W l.
   induction l.
@@ -421,31 +421,31 @@ Proof.
       rewrite <- H1.
       rewrite H.
       simpl nlist_list_pa.
-      rewrite altered_Ip_list_cons.
-      rewrite altered_Ip_eq.
+      rewrite alt_Ip_list_cons.
+      rewrite alt_Ip_eq.
       specialize (IHl pa_l1 pa_hat (Pred Qm) Ip).
       destruct IHl as [pa2 [pa_l2 IHl']].
 
       exists pa2.
       exists (consn_pa W (length l) pa_hat pa_l2).
       simpl nlist_list_pa.
-      rewrite altered_Ip_list_cons.
+      rewrite alt_Ip_list_cons.
       rewrite <- IHl'.
-      rewrite altered_Ip_eq.
+      rewrite alt_Ip_eq.
       reflexivity.
 
       intros.
       pose proof ((EqNat.beq_nat_false Qm Pn) H0).
       rewrite H.
       simpl nlist_list_pa.
-      rewrite altered_Ip_list_cons.
-      rewrite <- altered_Ip_switch.
+      rewrite alt_Ip_list_cons.
+      rewrite <- alt_Ip_switch.
       specialize (IHl pa_l1 pa_hat (Pred Pn) Ip).
       destruct IHl as [pa2 [pa_l2 IHl']].
       rewrite IHl'.
       assert (S (length l) = length (cons (Pred Pn) l)).
         simpl; reflexivity.
-      rewrite <- altered_Ip_list_cons.
+      rewrite <- alt_Ip_list_cons.
       exists pa2.
       exists (consn_pa W (length l) pa1 pa_l2).
       reflexivity.
@@ -457,11 +457,11 @@ Lemma alt_alt_list_2 : forall (W : Set) (Ip : predicate -> W -> Prop) (P : predi
                             (l : list predicate) (pa_l_hat : nlist_pa W (length l)) 
                             (pa_hat : W -> Prop),
    exists (pa : W -> Prop) (pa_l : nlist_pa W (length l)),
-     (altered_Ip (altered_Ip_list Ip (nlist_list_pa W (length l) pa_l) l) pa P) = 
-        (altered_Ip_list (altered_Ip Ip pa_hat P) (nlist_list_pa W (length l) pa_l_hat) l).
+     (alt_Ip (alt_Ip_list Ip (nlist_list_pa W (length l) pa_l) l) pa P) = 
+        (alt_Ip_list (alt_Ip Ip pa_hat P) (nlist_list_pa W (length l) pa_l_hat) l).
 Proof.
   intros.
-  rewrite altered_Ip_list_tail.
+  rewrite alt_Ip_list_tail.
   induction l.
     simpl length in *.
     assert (pa_l_hat = niln_pa W).
@@ -481,7 +481,7 @@ Proof.
     simpl.
     destruct a as [Qm].
     destruct P as [Pn].
-    rewrite altered_Ip_list_app.
+    rewrite alt_Ip_list_app.
     specialize (IHl pa_l1).
     destruct IHl as [pa2 [pa_l2 IHl']].
     case_eq (EqNat.beq_nat Qm Pn).
@@ -495,12 +495,12 @@ Proof.
         apply nlist_list_cons.
       simpl length in list_cons.
       rewrite list_cons.
-      rewrite altered_Ip_list_cons.
-      rewrite altered_Ip_list_app in IHl'.
+      rewrite alt_Ip_list_cons.
+      rewrite alt_Ip_list_app in IHl'.
       rewrite list_cons in IHl'.
-      rewrite altered_Ip_list_cons in IHl'.
-      rewrite altered_Ip_list_nil.
-      rewrite altered_Ip_list_nil in IHl'.
+      rewrite alt_Ip_list_cons in IHl'.
+      rewrite alt_Ip_list_nil.
+      rewrite alt_Ip_list_nil in IHl'.
       rewrite H0.
       rewrite <- IHl'.
       exists pa1. 
@@ -510,7 +510,7 @@ Proof.
         apply nlist_list_cons.
       simpl length in list_cons2.
       rewrite list_cons2.
-      rewrite altered_Ip_list_cons.
+      rewrite alt_Ip_list_cons.
       reflexivity.
 
       intros.
@@ -521,11 +521,11 @@ Proof.
         apply nlist_list_cons.  
       simpl length in list_cons.
       rewrite list_cons.
-      rewrite altered_Ip_list_app in IHl'.
+      rewrite alt_Ip_list_app in IHl'.
       simpl nlist_list_pa in IHl'.
-      rewrite altered_Ip_list_cons in IHl'.
-      simpl altered_Ip_list in IHl' at 3.
-      rewrite altered_Ip_list_cons.
+      rewrite alt_Ip_list_cons in IHl'.
+      simpl alt_Ip_list in IHl' at 3.
+      rewrite alt_Ip_list_cons.
       assert ((nlist_list_pa W (length (cons (Pred Pn) nil)) 
               (consn_pa W (length (nil: list predicate)) pa_hat (niln_pa W)))
                  = cons pa_hat (nlist_list_pa W (length (nil:list predicate)) (niln_pa W)))
@@ -533,11 +533,11 @@ Proof.
         apply nlist_list_cons.
       simpl length in list_cons2.
       rewrite list_cons2.
-      rewrite altered_Ip_list_cons.
+      rewrite alt_Ip_list_cons.
       unfold nlist_list_pa at 2.
-      unfold altered_Ip_list at 3.
+      unfold alt_Ip_list at 3.
       rewrite <- IHl'.
-      apply altered_Ip_switch.
+      apply alt_Ip_switch.
       pose proof ((EqNat.beq_nat_false Qm Pn) H).
       unfold not; intros.
       symmetry in H1.
@@ -549,19 +549,19 @@ Lemma nlist_list_closed_SO : forall (W : Set) (Iv : FOvariable -> W)
                            (Ip: predicate -> W -> Prop),
      SOturnst W Iv Ip Ir (list_closed_SO alpha l) <->
    forall pa_l : (nlist_pa W (length l)),
-      SOturnst W Iv (altered_Ip_list Ip (nlist_list_pa W (length l) pa_l) l) Ir alpha.
+      SOturnst W Iv (alt_Ip_list Ip (nlist_list_pa W (length l) pa_l) l) Ir alpha.
 Proof.
   intros W Iv Ir alpha l.
   induction l.
     simpl.
     split.
       intros H pa_l.
-      rewrite altered_Ip_list_nil.
+      rewrite alt_Ip_list_nil.
       exact H.
 
       intros H.
       specialize (H (niln_pa W)).
-      rewrite altered_Ip_list_nil in H.
+      rewrite alt_Ip_list_nil in H.
       exact H.
 
     intros.
@@ -573,10 +573,10 @@ Proof.
       destruct H0 as [pa1 [pa_l1 H0]].
       rewrite H0.
       simpl nlist_list_pa.
-      simpl altered_Ip_list.
+      simpl alt_Ip_list.
       assert (exists (pa : W -> Prop) (pa_l : nlist_pa W (length l)),
-            (altered_Ip (altered_Ip_list Ip (nlist_list_pa W (length l) pa_l1) l) pa1 a) = 
-            (altered_Ip_list (altered_Ip Ip pa a) (nlist_list_pa W (length l) pa_l) l)).
+            (alt_Ip (alt_Ip_list Ip (nlist_list_pa W (length l) pa_l1) l) pa1 a) = 
+            (alt_Ip_list (alt_Ip Ip pa a) (nlist_list_pa W (length l) pa_l) l)).
         apply alt_alt_list_1.
       destruct H1 as [pa2 [pa_l2 H1]].
       rewrite H1.
@@ -594,9 +594,9 @@ Proof.
       intros.
       simpl in H.
       assert (exists (pred_asgmt1 : W -> Prop) (pa_l1 : nlist_pa W (length l)),
-           (altered_Ip (altered_Ip_list Ip (nlist_list_pa W (length l) pa_l1) l)
+           (alt_Ip (alt_Ip_list Ip (nlist_list_pa W (length l) pa_l1) l)
               pred_asgmt1 a) = 
-           (altered_Ip_list (altered_Ip Ip pred_asgmt a) 
+           (alt_Ip_list (alt_Ip Ip pred_asgmt a) 
               (nlist_list_pa W (length l) pa_l) l)).
          apply alt_alt_list_2.
        destruct H0 as [pred_asgmt1 [pa_l1 H0]].
@@ -819,12 +819,12 @@ Proof.
         apply H.
 Qed.
 
-Lemma same_altered_rem : forall (W:Set) (l : list predicate)
+Lemma same_alt_rem : forall (W:Set) (l : list predicate)
                             (Ip Ip': predicate -> W -> Prop) 
                             (n : nat) (pred_asgmt : W -> Prop) ,
   same_Ip_list W Ip Ip' (list_rem l n) <-> 
-    same_Ip_list W (altered_Ip Ip pred_asgmt (Pred n)) 
-                   (altered_Ip Ip' pred_asgmt (Pred n)) l.
+    same_Ip_list W (alt_Ip Ip pred_asgmt (Pred n)) 
+                   (alt_Ip Ip' pred_asgmt (Pred n)) l.
 Proof.
   intros W l.
   induction l.
@@ -842,13 +842,13 @@ Proof.
         intros.
         pose proof (EqNat.beq_nat_true n n0 H0).
         rewrite H1 in *.
-        simpl altered_Ip.
+        simpl alt_Ip.
         rewrite <- EqNat.beq_nat_refl.
         reflexivity.
 
         intros.
         pose proof (EqNat.beq_nat_false n n0 H0).
-        unfold altered_Ip.
+        unfold alt_Ip.
         rewrite H0.
         simpl in H.
         rewrite H0 in H.
@@ -1028,8 +1028,8 @@ Proof.
     rewrite same_cons in *. 
     rewrite SOturnst_allSO in *.
     intros.
-    apply IHalpha with (Ip := (altered_Ip Ip pred_asgmt (Pred n))).
-      apply same_altered_rem.
+    apply IHalpha with (Ip := (alt_Ip Ip pred_asgmt (Pred n))).
+      apply same_alt_rem.
       apply same_rem.
       apply H.
 
@@ -1042,8 +1042,8 @@ Proof.
     exists pred_asgmt.
     simpl preds_in in H.
     rewrite same_cons in H.
-    apply IHalpha with (Ip := (altered_Ip Ip pred_asgmt (Pred n))).
-    apply same_altered_rem.
+    apply IHalpha with (Ip := (alt_Ip Ip pred_asgmt (Pred n))).
+    apply same_alt_rem.
       apply same_rem.
       apply H.
 
@@ -1083,8 +1083,8 @@ Proof.
     rewrite SOturnst_allSO in *.
     intros.
     specialize (H0 pred_asgmt).
-    apply IHl with (Ip := (altered_Ip Ip pred_asgmt (Pred n))).
-      apply same_altered_rem.
+    apply IHl with (Ip := (alt_Ip Ip pred_asgmt (Pred n))).
+      apply same_alt_rem.
       rewrite <- list_without_rem.
       exact H.
 
