vsSahlq/Coq code/vsSahlq_instant13.v
@@ -859,7 +859,7 @@ Lemma equiv_new_simpl3_lP : forall lP llv x alpha W Iv Ip Ir pa0,
   @consistent_lP_lpa _ pa0 lP (vsS_pa_l Iv llv (list_Var (length lP) x)) ->
   ex_attached_allFO_llv alpha llv = false ->
   ex_attached_exFO_llv alpha llv = false ->
-    SOturnst W Iv (altered_Ip_list Ip (vsS_pa_l Iv llv (list_Var (length lP) x)) lP) Ir alpha <->
+    SOturnst W Iv (alt_Ip_list Ip (vsS_pa_l Iv llv (list_Var (length lP) x)) lP) Ir alpha <->
     SOturnst W Iv Ip Ir (replace_pred_l alpha lP (list_Var (length lP) x) (vsS_syn_l llv x)).
 Proof.
   induction lP; intros llv x alpha W Iv Ip Ir pa0 Hl Hno Hcon Hind Hat1 Hat2.
@@ -964,7 +964,7 @@ Qed.
       (vsS_pa_l Iv llv (list_Var (length lP) x)) = constant_l pa n) ->
   ex_attached_allFO_llv alpha llv = false ->
   ex_attached_exFO_llv alpha llv = false ->
-    SOturnst W Iv (altered_Ip_list Ip (vsS_pa_l Iv llv (list_Var (length lP) x)) lP) Ir alpha <->
+    SOturnst W Iv (alt_Ip_list Ip (vsS_pa_l Iv llv (list_Var (length lP) x)) lP) Ir alpha <->
     SOturnst W Iv Ip Ir (replace_pred_l alpha lP (list_Var (length lP) x) (vsS_syn_l llv x)).
 Proof.
   induction lP; intros llv x alpha W Iv Ip Ir Hl Hno Hcon Hind Hat1 Hat2.
@@ -1155,8 +1155,8 @@ Qed.
 Lemma alt_alt_list_1' : forall (W : Set) (l : list predicate) (pa_l_hat : nlist (length l)) 
                             (pa_hat : W -> Prop) (P : predicate) (Ip : predicate -> W -> Prop) ,
       exists (pa : W -> Prop) (pa_l : nlist (length l)),
-          (altered_Ip (altered_Ip_list Ip (nlist_list (length l) pa_l_hat) l) pa_hat P) 
-        = (altered_Ip_list (@altered_Ip W Ip pa P) (nlist_list (length l) pa_l) l).
+          (alt_Ip (alt_Ip_list Ip (nlist_list (length l) pa_l_hat) l) pa_hat P) 
+        = (alt_Ip_list (@alt_Ip W Ip pa P) (nlist_list (length l) pa_l) l).
 Proof.
   intros W l.
   induction l.
@@ -1185,31 +1185,31 @@ Proof.
       rewrite <- H1.
       rewrite H.
       simpl nlist_list.
-      rewrite altered_Ip_list_cons.
-      rewrite altered_Ip_eq.
+      rewrite alt_Ip_list_cons.
+      rewrite alt_Ip_eq.
       specialize (IHl pa_l1 pa_hat (Pred Qm) Ip).
       destruct IHl as [pa2 [pa_l2 IHl']].
 
       exists pa2.
       exists (consn (length l) pa_hat pa_l2).
       simpl nlist_list.
-      rewrite altered_Ip_list_cons.
+      rewrite alt_Ip_list_cons.
       rewrite <- IHl'.
-      rewrite altered_Ip_eq.
+      rewrite alt_Ip_eq.
       reflexivity.
 
       intros.
       pose proof ((EqNat.beq_nat_false Qm Pn) H0).
       rewrite H.
       simpl nlist_list.
-      rewrite altered_Ip_list_cons.
-      rewrite <- altered_Ip_switch.
+      rewrite alt_Ip_list_cons.
+      rewrite <- alt_Ip_switch.
       specialize (IHl pa_l1 pa_hat (Pred Pn) Ip).
       destruct IHl as [pa2 [pa_l2 IHl']].
       rewrite IHl'.
       assert (S (length l) = length (cons (Pred Pn) l)).
         simpl; reflexivity.
-      rewrite <- altered_Ip_list_cons.
+      rewrite <- alt_Ip_list_cons.
       exists pa2.
       exists (consn (length l) pa1 pa_l2).
       reflexivity.
@@ -1217,11 +1217,11 @@ Proof.
         exact H1.
 Qed.
 
-Lemma altered_Ip_list_tail' : forall (W : Set) (Ip : predicate -> W -> Prop) (P : predicate)
+Lemma alt_Ip_list_tail' : forall (W : Set) (Ip : predicate -> W -> Prop) (P : predicate)
                             (l : list predicate) (pa_l : nlist (length l)) 
                             (pa: W -> Prop),
-         altered_Ip_list (altered_Ip Ip pa P) (nlist_list (length l) pa_l) l
-            = altered_Ip_list Ip (app (nlist_list (length l) pa_l) (cons pa nil) ) (app l (cons P nil)).
+         alt_Ip_list (alt_Ip Ip pa P) (nlist_list (length l) pa_l) l
+            = alt_Ip_list Ip (app (nlist_list (length l) pa_l) (cons pa nil) ) (app l (cons P nil)).
 Proof.
   intros.
   induction l.
@@ -1243,11 +1243,11 @@ Proof.
     reflexivity.
 Qed.
 
-Lemma altered_Ip_list_app' : forall (W : Set) (Ip : predicate -> W -> Prop) (P : predicate)
+Lemma alt_Ip_list_app' : forall (W : Set) (Ip : predicate -> W -> Prop) (P : predicate)
                             (l : list predicate) (pa_l : nlist (length l)) 
                             (pa : W -> Prop),
-       (altered_Ip_list Ip (app (nlist_list (length l) pa_l) (cons pa nil)) (l ++ P :: nil))
-     = (altered_Ip_list (altered_Ip_list Ip (nlist_list 1 (consn 0 pa (niln)))
+       (alt_Ip_list Ip (app (nlist_list (length l) pa_l) (cons pa nil)) (l ++ P :: nil))
+     = (alt_Ip_list (alt_Ip_list Ip (nlist_list 1 (consn 0 pa (niln)))
           (P :: nil)) (nlist_list (length l) pa_l) l).
 Proof.
   intros.
@@ -1286,11 +1286,11 @@ Lemma alt_alt_list_2' : forall (W : Set) (Ip : predicate -> W -> Prop) (P : pred
                             (l : list predicate) (pa_l_hat : nlist (length l)) 
                             (pa_hat : W -> Prop),
    exists (pa : W -> Prop) (pa_l : nlist (length l)),
-     (altered_Ip (altered_Ip_list Ip (nlist_list (length l) pa_l) l) pa P) = 
-        (altered_Ip_list (altered_Ip Ip pa_hat P) (nlist_list (length l) pa_l_hat) l).
+     (alt_Ip (alt_Ip_list Ip (nlist_list (length l) pa_l) l) pa P) = 
+        (alt_Ip_list (alt_Ip Ip pa_hat P) (nlist_list (length l) pa_l_hat) l).
 Proof.
   intros.
-  rewrite altered_Ip_list_tail'.
+  rewrite alt_Ip_list_tail'.
   induction l.
     simpl length in *.
     assert (pa_l_hat = niln).
@@ -1310,7 +1310,7 @@ Proof.
     simpl.
     destruct a as [Qm].
     destruct P as [Pn].
-    rewrite altered_Ip_list_app'.
+    rewrite alt_Ip_list_app'.
     specialize (IHl pa_l1).
     destruct IHl as [pa2 [pa_l2 IHl']].
     case_eq (EqNat.beq_nat Qm Pn).
@@ -1324,12 +1324,12 @@ Proof.
         apply nlist_list_cons'.
       simpl length in list_cons.
       rewrite list_cons.
-      rewrite altered_Ip_list_cons.
-      rewrite altered_Ip_list_app' in IHl'.
+      rewrite alt_Ip_list_cons.
+      rewrite alt_Ip_list_app' in IHl'.
       rewrite list_cons in IHl'.
-      rewrite altered_Ip_list_cons in IHl'.
-      rewrite altered_Ip_list_nil.
-      rewrite altered_Ip_list_nil in IHl'.
+      rewrite alt_Ip_list_cons in IHl'.
+      rewrite alt_Ip_list_nil.
+      rewrite alt_Ip_list_nil in IHl'.
       rewrite H0.
       rewrite <- IHl'.
       exists pa1. 
@@ -1339,7 +1339,7 @@ Proof.
         apply nlist_list_cons'.
       simpl length in list_cons2.
       rewrite list_cons2.
-      rewrite altered_Ip_list_cons.
+      rewrite alt_Ip_list_cons.
       reflexivity.
 
       intros.
@@ -1350,11 +1350,11 @@ Proof.
         apply nlist_list_cons'.  
       simpl length in list_cons.
       rewrite list_cons.
-      rewrite altered_Ip_list_app' in IHl'.
+      rewrite alt_Ip_list_app' in IHl'.
       simpl nlist_list in IHl'.
-      rewrite altered_Ip_list_cons in IHl'.
-      simpl altered_Ip_list in IHl' at 3.
-      rewrite altered_Ip_list_cons.
+      rewrite alt_Ip_list_cons in IHl'.
+      simpl alt_Ip_list in IHl' at 3.
+      rewrite alt_Ip_list_cons.
       assert ((nlist_list (length (cons (Pred Pn) nil)) 
               (consn (length (nil: list predicate)) pa_hat (niln)))
                  = cons pa_hat (nlist_list (length (nil:list predicate)) (niln)))
@@ -1362,11 +1362,11 @@ Proof.
         apply nlist_list_cons'.
       simpl length in list_cons2.
       rewrite list_cons2.
-      rewrite altered_Ip_list_cons.
+      rewrite alt_Ip_list_cons.
       unfold nlist_list at 2.
-      unfold altered_Ip_list at 3.
+      unfold alt_Ip_list at 3.
       rewrite <- IHl'.
-      apply altered_Ip_switch.
+      apply alt_Ip_switch.
       pose proof ((EqNat.beq_nat_false Qm Pn) H).
       unfold not; intros.
       symmetry in H1.
@@ -1378,19 +1378,19 @@ Lemma  nlist_list_closed_SO'  : forall (W : Set) (Iv : FOvariable -> W)
                            (Ip: predicate -> W -> Prop),
      SOturnst W Iv Ip Ir (list_closed_SO alpha l) <->
    forall pa_l : (nlist (length l)),
-      SOturnst W Iv (altered_Ip_list Ip (nlist_list (length l) pa_l) l) Ir alpha.
+      SOturnst W Iv (alt_Ip_list Ip (nlist_list (length l) pa_l) l) Ir alpha.
 Proof.
   intros W Iv Ir alpha l.
   induction l.
     simpl.
     split.
       intros H pa_l.
-      rewrite altered_Ip_list_nil.
+      rewrite alt_Ip_list_nil.
       exact H.
 
       intros H.
       specialize (H (niln)).
-      rewrite altered_Ip_list_nil in H.
+      rewrite alt_Ip_list_nil in H.
       exact H.
 
     intros.
@@ -1402,10 +1402,10 @@ Proof.
       destruct H0 as [pa1 [pa_l1 H0]].
       rewrite H0.
       simpl nlist_list_pa.
-      simpl altered_Ip_list.
+      simpl alt_Ip_list.
       assert (exists (pa : W -> Prop) (pa_l : nlist (length l)),
-            (altered_Ip (altered_Ip_list Ip (nlist_list (length l) pa_l1) l) pa1 a) = 
-            (altered_Ip_list (altered_Ip Ip pa a) (nlist_list (length l) pa_l) l)).
+            (alt_Ip (alt_Ip_list Ip (nlist_list (length l) pa_l1) l) pa1 a) = 
+            (alt_Ip_list (alt_Ip Ip pa a) (nlist_list (length l) pa_l) l)).
         apply alt_alt_list_1'.
       destruct H1 as [pa2 [pa_l2 H1]].
       rewrite H1.
@@ -1423,9 +1423,9 @@ Proof.
       intros.
       simpl in H.
       assert (exists (pred_asgmt1 : W -> Prop) (pa_l1 : nlist (length l)),
-           (altered_Ip (altered_Ip_list Ip (nlist_list (length l) pa_l1) l)
+           (alt_Ip (alt_Ip_list Ip (nlist_list (length l) pa_l1) l)
               pred_asgmt1 a) = 
-           (altered_Ip_list (altered_Ip Ip pred_asgmt a) 
+           (alt_Ip_list (alt_Ip Ip pred_asgmt a) 
               (nlist_list (length l) pa_l) l)).
          apply alt_alt_list_2'.
        destruct H0 as [pred_asgmt1 [pa_l1 H0]].
